Add support for specifying naming conventions
We can now specify how functions and types should be cased, as well as
specifying package and class names.  There is some support for
specifying variable casing, but that's not really plugged in anywhere
yet.  Perhaps it should be removed?

src/Stringification/Language.v
@@ -20,6 +20,7 @@ Require Import Crypto.Util.MSets.Iso.
 Require Import Crypto.Util.MSets.Sum.
 Require Import Crypto.Util.Strings.Decimal.
 Require Import Crypto.Util.Strings.Show.
+Require Import Crypto.Util.Strings.NamingConventions.
 Require Import Crypto.Util.ZRange.
 Require Import Crypto.Util.ZRange.Operations.
 Require Import Crypto.Util.ZRange.Show.
@@ -50,6 +51,50 @@ Module Compilers.
     (** How to relax zranges *)
     Class relax_zrange_opt := relax_zrange : zrange -> zrange.
     Typeclasses Opaque relax_zrange_opt.
+    (** What's the package name? *)
+    Class package_name_opt := internal_package_name : option string.
+    Typeclasses Opaque package_name_opt.
+    (** What's the class name? *)
+    Class class_name_opt := internal_class_name : option string.
+    Typeclasses Opaque class_name_opt.
+    Class language_naming_conventions_opt :=
+      { public_function_naming_convention : option capitalization_convention
+        ; private_function_naming_convention : option capitalization_convention
+        ; public_type_naming_convention : option capitalization_convention
+        ; private_type_naming_convention : option capitalization_convention
+        ; variable_naming_convention : option capitalization_convention
+        ; package_naming_convention : option capitalization_convention
+        ; class_naming_convention : option capitalization_convention
+      }.
+    Definition default_language_naming_conventions : language_naming_conventions_opt
+      := {| public_function_naming_convention := None
+            ; private_function_naming_convention := None
+            ; public_type_naming_convention := None
+            ; private_type_naming_convention := None
+            ; variable_naming_convention := None
+            ; package_naming_convention := None
+            ; class_naming_convention := None
+         |}.
+
+    Definition convert_to_naming_convention (convention : option capitalization_convention) (s : string) : string
+      := match convention with
+         | Some convention => convert_case snake_case convention s
+         | None => s
+         end.
+    Definition package_name {pkg_name : package_name_opt} {language_naming_conventions : language_naming_conventions_opt} (prefix : string) : string
+      := match pkg_name with
+         | Some name => name
+         | None => convert_to_naming_convention
+                     package_naming_convention
+                     (if String.endswith "_" prefix then substring 0 (String.length prefix - 1) prefix else prefix)
+         end.
+    Definition class_name {cls_name : class_name_opt} {language_naming_conventions : language_naming_conventions_opt} (prefix : string) : string
+      := match cls_name with
+         | Some name => name
+         | None => convert_to_naming_convention
+                     class_naming_convention
+                     (if String.endswith "_" prefix then substring 0 (String.length prefix - 1) prefix else prefix)
+         end.
   End Options.
 
   Module ToString.
@@ -756,6 +801,24 @@ Module Compilers.
                 with_parens
                 ((if is_unsigned t then "u" else "") ++ "int" ++ Decimal.Z.to_string (bitwidth_of t)).
 
+      Definition to_string_gen
+                 {language_naming_conventions : language_naming_conventions_opt}
+                 (standard_bitwidths : list Z)
+                 (unsigned_s signed_s : string)
+                 (standard_postfix special_postfix : string)
+                 (private : bool) (prefix : string)
+                 (t : type)
+        : string
+        := let is_standard := existsb (Z.eqb (bitwidth_of t)) standard_bitwidths in
+           (if is_standard
+            then (fun s => s)
+            else (fun s => convert_to_naming_convention
+                             (if private then private_type_naming_convention else public_type_naming_convention)
+                             (prefix ++ s)))
+             ((if is_unsigned t then unsigned_s else signed_s)
+                ++ Decimal.Z.to_string (ToString.int.bitwidth_of t)
+                ++ (if is_standard then standard_postfix else special_postfix)).
+
       Definition union (t1 t2 : type) : type := of_zrange_relaxed (ZRange.union (to_zrange t1) (to_zrange t2)).
 
       Definition union_zrange (r : zrange) (t : type) : type
@@ -1129,6 +1192,26 @@ Module Compilers.
            end%list.
     End OfPHOAS.
 
+    Definition format_special_function_name
+               {language_naming_conventions : language_naming_conventions_opt}
+               (internal_private : bool)
+               (prefix : string)
+               (name : string)
+               (is_signed : bool)
+               (bw : Z)
+      : string
+      := convert_to_naming_convention
+           (if internal_private then private_function_naming_convention else public_function_naming_convention)
+           (prefix ++ name ++ "_" ++ (if negb is_signed then "u" else "") ++ Decimal.Z.to_string bw).
+    Definition format_special_function_name_ty
+               {language_naming_conventions : language_naming_conventions_opt}
+               (internal_private : bool)
+               (prefix : string)
+               (name : string)
+               (t : int.type)
+      : string
+      := format_special_function_name internal_private prefix name (int.is_signed t) (int.bitwidth_of t).
+
     Definition preprocess_comment_block (lines : list string)
       := String.split String.NewLine (String.concat String.NewLine lines).
 
@@ -1154,15 +1237,11 @@ Module Compilers.
             lines)]. *)
         comment_file_header_block : list string -> list string;
 
-        (** Convert the name of a function from
-            lowercase_with_underscores to whatever convention the
-            language uses *)
-        adjust_name : forall (static : bool) (name : string), string;
-
         (** Converts a PHOAS AST to lines of code * info on which
             primitive functions are called, or else an error string *)
         ToFunctionLines
         : forall {relax_zrange : relax_zrange_opt}
+                 {language_naming_conventions : language_naming_conventions_opt}
                  (machine_wordsize : Z)
                  (do_bounds_check : bool) (internal_static : bool) (static : bool) (prefix : string) (name : string)
                  {t}
@@ -1175,12 +1254,18 @@ Module Compilers.
 
         (** Generates a header of any needed typedefs, etc based on the idents used and the curve-specific prefix *)
         header
-        : forall (machine_wordsize : Z) (static : bool) (prefix : string) (ident_info : ident_infos),
+        : forall {language_naming_conventions : language_naming_conventions_opt}
+                 {package_name : package_name_opt}
+                 {class_name : class_name_opt}
+                 (machine_wordsize : Z) (internal_static : bool) (static : bool) (prefix : string) (ident_info : ident_infos),
             list string;
 
         (** The footer on the file, if any *)
         footer
-        : forall (machine_wordsize : Z) (static : bool) (prefix : string) (ident_info : ident_infos),
+        : forall {language_naming_conventions : language_naming_conventions_opt}
+                 {package_name : package_name_opt}
+                 {class_name : class_name_opt}
+                 (machine_wordsize : Z) (internal_static : bool) (static : bool) (prefix : string) (ident_info : ident_infos),
             list string;
 
         (** Filters [ident_infos] to strip out primitive functions
