src/SlowPrimeSynthesisExamples.v
@@ -39,6 +39,9 @@ Local Coercion Z.pos : positive >-> Z.
 Local Existing Instance default_low_level_rewriter_method.
 Local Instance : unfold_value_barrier_opt := true.
 Local Instance : tight_upperbound_fraction_opt := default_tight_upperbound_fraction.
+Local Existing Instance default_language_naming_conventions.
+Local Instance : package_name_opt := None.
+Local Instance : class_name_opt := None.
 
 Module debugging_21271_from_bytes.
   Import Crypto.PushButtonSynthesis.UnsaturatedSolinas.
