src/Stringification/JSON.v
@@ -360,6 +360,7 @@ Module JSON.
 
   Definition ToFunctionLines
              {relax_zrange : relax_zrange_opt}
+             {language_naming_conventions : language_naming_conventions_opt}
              (machine_wordsize : Z)
              (do_bounds_check : bool) (internal_static : bool) (static : bool) (prefix : string) (name : string)
              {t}
@@ -388,10 +389,9 @@ Module JSON.
   Definition OutputJSONAPI : ToString.OutputLanguageAPI :=
     {| ToString.comment_block _ := [];
        ToString.comment_file_header_block _ := [];
-       ToString.adjust_name _ name := name;
        ToString.ToFunctionLines := @ToFunctionLines;
-       ToString.header := fun _ _ _ _ => [];
-       ToString.footer := fun _ _ _ _ => [];
+       ToString.header := fun _ _ _ _ _ _ _ _ => [];
+       ToString.footer := fun _ _ _ _ _ _ _ _ => [];
        (** No special handling for any functions *)
        ToString.strip_special_infos machine_wordsize infos := infos |}.
 
